\documentclass{article}
\usepackage{geometry}
\geometry{%
  paperwidth=9.72cm,
  paperheight=10.76cm,
  margin=5mm
}
\usepackage{amsmath}
\begin{document}

\begin{align*}
  1-\frac{x}{1 !}+\frac{x(x-1)}{2 !}-\frac{x(x-1)(x-2)}{3 !}=\frac{(x-1)(x-2)}{2}-\frac{x(x-1)(x-2)}{6}=-\frac{(x-1)(x-2)(x-3)}{3 !}
\end{align*}

\begin{multline*}
  1-\frac{x}{1 !}+\frac{x(x-1)}{2 !}-\frac{x(x-1)(x-2)}{3 !}=\\
  =\frac{(x-1)(x-2)}{2}-\frac{x(x-1)(x-2)}{6}=\\
  =-\frac{(x-1)(x-2)(x-3)}{3 !}
\end{multline*}

\end{document}
