\documentclass{article}
\usepackage{amsmath}

\begin{document}

Superíndice: $x^{23}$

Subíndice: $H_2O$

Superíndice y subíndice: $x^4_2$

$\frac{abc}{12}$

$\sqrt{\frac{a}{b}}$

$\int_{x_0}^{x}f(x)dx$

$\sum_{i=1}^{n}i^2$


\begin{equation}\label{eq:prueba}
  x^2 + y^2 = z^2
\end{equation}
\begin{equation*}
  x^2 + y^2 = z^2
\end{equation*}

Ecuación \ref{eq:prueba}

\begin{equation}
  \left[
  \begin{array}{ccc}
    x & y & z \\
    1 & 2 & 3
  \end{array}
  \right]
\end{equation}

\begin{equation}
  \left\{
    \begin{array}{l}
      x + y = 43 \\
      x - y = 23
    \end{array}
  \right.
\end{equation}

\begin{equation}
  \begin{matrix}
    x & y & z \\
    1 & 2 & 3\\
    4 & 5 & 6
  \end{matrix}
\end{equation}

\begin{equation}
  \begin{pmatrix}
    x & y & z \\
    1 & 2 & 3\\
    4 & 5 & 6
  \end{pmatrix}
\end{equation}

\begin{equation}
  \begin{bmatrix}
    x & y & z \\
    1 & 2 & 3\\
    4 & 5 & 6
  \end{bmatrix}
\end{equation}


\begin{equation}
  \begin{vmatrix}
    x & y & z \\
    1 & 2 & 3\\
    4 & 5 & 6
  \end{vmatrix}
\end{equation}

\begin{equation}
  E = (ab)^2 \hspace{1cm} E = [ab]^2 \hspace{1cm} E = \{ab\}^2\\
\end{equation}

\begin{equation}
  E = \left(\sqrt{\sqrt{\sqrt{\sqrt{\sqrt{2}}}}}\right)
\end{equation}

\begin{equation}
  E = \left[\sqrt{\sqrt{\sqrt{\sqrt{\sqrt{2}}}}}\right]
\end{equation}


\begin{equation*}
  abc   m \text{abc      m} \hspace{1cm} \mbox{abc m}  
\end{equation*}

\begin{equation*}
  abc \; m
\end{equation*}
\begin{equation*}
  abc \, m
\end{equation*}
\begin{equation*}
  abc \! m
\end{equation*}
\begin{equation*}
  abc \qquad m
\end{equation*}
\begin{equation*}
  abc \hspace{1cm} m
\end{equation*}



\begin{align*}
  a + b + \cdots + m\\
  a + b + \ldots + m\\
  \vdots \\
  \ddots
\end{align*}

\begin{align*}
  \hat{a} \hat{u} \hat{i} \\
  \vec{a} \vec{m} \vec{np} \\
  \bar{a} \overline{m}
\end{align*}


\begin{align*}
  E &= \underbrace{a + b + \cdots + m}_{\text{suma}}\\
  E &= \overbrace{a + b + \cdots + m}^{\text{suma}}
\end{align*}

\begin{align*}
  \sin 45^{\circ} \cos   \tan   \cot   \sec   \csc \\
  \log \det \ln
\end{align*}

\begin{align*}
  \alpha \beta \gamma
\end{align*}


% \begin{nombreEntorno}
%   &
% \end{nombreEntorno}

\begin{align*}
  expresion &= expresion    &   expresion &= expresion\\
  x^2 + y^2 &= r^2          &   y - y_0 &= m(x - x_0)
\end{align*}


\begin{multline*}
  1-\frac{x}{1 !}+\frac{x(x-1)}{2 !}-\frac{x(x-1)(x-2)}{3 !}= \\ 
  =\frac{(x-1)(x-2)}{2}-\frac{x(x-1)(x-2)}{6}=\\
  =-\frac{(x-1)(x-2)(x-3)}{3 !}-\frac{(x-1)(x-2)(x-3)}{3 !}
\end{multline*}
\end{document}
